Tidied up a bit more

formal/find_unused_defs.py
@@ -15,7 +15,7 @@ dec_re = re.compile("(definition|fun|function|abbreviation) \"?(\w+) (\w|=)")
 
 
 def find_unused_defs(path):
-    print(path)
+    defs = []
     with open(path) as f:
         content = f.readlines()
         joined = "\n".join(content)
@@ -23,15 +23,17 @@ def find_unused_defs(path):
             match = def_re.search(line)
             if match is not None:
                 if joined.count(match.group(2)) < 3:
-                    print(" ", match.group(2))
+                    defs.append(match.group(2))
+    return defs
                     
 
-path = "./inference/heuristics/PTA_Generalisation.thy"
-find_unused_defs(path)
-
-# for root, dirs, files in os.walk(".", topdown=False):
-#     files = [f for f in files if f.endswith(".thy")]
-#     for name in files:
-#         path = os.path.join(root, name)
-#         find_unused_defs(path)
+for root, dirs, files in os.walk(".", topdown=False):
+    files = [f for f in files if f.endswith(".thy")]
+    for name in files:
+        path = os.path.join(root, name)
+        defs = find_unused_defs(path)
+        if defs:
+            print(path)
+            for d in defs:
+                print("  ", d)
         
