formal/inference/heuristics/Same_Register.thy
@@ -1,49 +1,40 @@
 theory Same_Register
   imports "../Inference"
 begin
-
-fun updates :: "update_function list \<Rightarrow> vname option" where
-  "updates [(n, a)] = Some (R n)" |
-  "updates _ = None"
-
-fun a_replace_with :: "vname aexp \<Rightarrow> nat \<Rightarrow> nat \<Rightarrow> vname aexp" where
-  "a_replace_with (L v) _ _ = L v" |
-  "a_replace_with (V v) r1 r2 = (if v = R r1 then V (R r2) else V v)" |
-  "a_replace_with (Plus a1 a2) r1 r2 = Plus (a_replace_with a1 r1 r2) (a_replace_with a2 r1 r2)" |
-  "a_replace_with (Minus a1 a2) r1 r2 = Minus (a_replace_with a1 r1 r2) (a_replace_with a2 r1 r2)" |
-  "a_replace_with (Times a1 a2) r1 r2 = Times (a_replace_with a1 r1 r2) (a_replace_with a2 r1 r2)"
-
-fun g_replace_with :: "vname gexp \<Rightarrow> nat \<Rightarrow> nat \<Rightarrow> vname gexp" where
-  "g_replace_with (Bc x) _ _ = gexp.Bc x" |
-  "g_replace_with (Eq a1 a2) r1 r2 = Eq (a_replace_with a1 r1 r2) (a_replace_with a2 r1 r2)" |
-  "g_replace_with (Gt a1 a2) r1 r2 = Eq (a_replace_with a1 r1 r2) (a_replace_with a2 r1 r2)" |
-  "g_replace_with (Nor g1 g2) r1 r2 = Nor (g_replace_with g1 r1 r2) (g_replace_with g2 r1 r2)" |
-  "g_replace_with (In v s) r1 r2 = In v s"
-
-(* replace r1 with r2 *)
-fun u_replace_with :: "update_function \<Rightarrow> nat \<Rightarrow> nat \<Rightarrow> update_function" where
-  "u_replace_with (r, a) r1 r2 = ((if r = r1 then r2 else r), a_replace_with a r1 r2)"
-
-definition t_replace_with :: "transition \<Rightarrow> nat \<Rightarrow> nat \<Rightarrow> transition" where
-  "t_replace_with t r1 r2 = \<lparr>Label = Label t,
-                             Arity = Arity t,
-                             Guards = map (\<lambda>g. g_replace_with g r1 r2) (Guards t),
-                             Outputs = map (\<lambda>p. a_replace_with p r1 r2) (Outputs t),
-                             Updates = map (\<lambda>u. u_replace_with u r1 r2) (Updates t)\<rparr>"
+text\<open>The \texttt{same_register} heuristic aims to replace registers which are used in the same way.\<close>
 
 definition replace_with :: "iEFSM \<Rightarrow> nat \<Rightarrow> nat \<Rightarrow> iEFSM" where
-  "replace_with e r1 r2 = (fimage (\<lambda>(u, tf, t). (u, tf, t_replace_with t r1 r2)) e)"
+  "replace_with e r1 r2 = (fimage (\<lambda>(u, tf, t). (u, tf,Transition.rename_regs (id(r1:=r2)) t)) e)"
+
+fun merge_if_same :: "iEFSM \<Rightarrow> (transition_matrix \<Rightarrow> bool) \<Rightarrow> (nat \<times> nat) list \<Rightarrow> iEFSM" where
+  "merge_if_same e _ [] = e" |
+  "merge_if_same e check ((r1, r2)#rs) = (
+    let transitions = fimage (snd \<circ> snd) e in
+    if \<exists>(t1, t2) |\<in>| ffilter (\<lambda>(t1, t2). t1 < t2) (transitions |\<times>| transitions).
+      same_structure t1 t2 \<and> r1 \<in> enumerate_regs t1 \<and> r2 \<in> enumerate_regs t2
+    then
+      let newE = replace_with e r1 r2 in
+      if check (tm newE) then
+        merge_if_same newE check rs
+      else
+        merge_if_same e check rs
+    else
+      merge_if_same e check rs
+  )"
+
+definition merge_regs :: "iEFSM \<Rightarrow> (transition_matrix \<Rightarrow> bool) \<Rightarrow> iEFSM" where
+  "merge_regs e check = (
+    let
+      regs = all_regs e;
+      reg_pairs = sorted_list_of_set (Set.filter (\<lambda>(r1, r2). r1 < r2) (regs \<times> regs))
+    in
+    merge_if_same e check reg_pairs
+  )"
 
 fun same_register :: update_modifier where
-  "same_register t1ID t2ID s new _ old _ = (let
-     t1 = get_by_ids new t1ID;
-     t2 = get_by_ids new t2ID;
-     ut1 = updates (Updates t1);
-     ut2 = updates (Updates t2) in
-     if same_structure t1 t2 then
-      case (ut1, ut2) of
-       (Some (R r1), Some (R r2)) \<Rightarrow> Some (replace_with new r1 r2) |
-       (_, _) \<Rightarrow> None
-     else None
+  "same_register t1ID t2ID s new _ old check = (
+    let new' = merge_regs new check in
+    if new' = new then None else Some new'
    )"
+
 end
