formal/inference/heuristics/Weak_Subsumption.thy
@@ -5,8 +5,8 @@ begin
 definition maxBy :: "('a \<Rightarrow> 'b::linorder) \<Rightarrow> 'a \<Rightarrow> 'a \<Rightarrow> 'a" where
   "maxBy f a b = (if (f a > f b) then a else b)"
 
-fun weak_subsumption :: "log \<Rightarrow> update_modifier" where
-  "weak_subsumption log t1ID t2ID s new _ old _ = (let
+fun weak_subsumption :: "update_modifier" where
+  "weak_subsumption t1ID t2ID s new _ old check = (let
      t1 = get_by_ids new t1ID;
      t2 = get_by_ids new t2ID
      in
@@ -18,13 +18,13 @@ fun weak_subsumption :: "log \<Rightarrow> update_modifier" where
         minT = if maxT = t1 then t2 else t1;
         newEFSMmax = replace_all new [t1ID, t2ID] maxT in
       \<comment> \<open>Most of the time, we'll want the transition with the most updates so start with that one\<close>
-      if satisfies (set log) (tm newEFSMmax) then
+      if check (tm newEFSMmax) then
         Some newEFSMmax
       else
         \<comment> \<open>There may be other occasions where we want to try the other transition\<close>
         \<comment> \<open>e.g. if their updates are equal but one has a different guard\<close>
         let newEFSMmin = replace_all new [t1ID, t2ID] minT in
-        if satisfies (set log) (tm newEFSMmin) then
+        if check (tm newEFSMmin) then
           Some newEFSMmin
         else
           None
